fstar/MLS.TreeKEM.Types.fst
@@ -6,20 +6,20 @@ open MLS.Tree
 
 #set-options "--fuel 0 --ifuel 0"
 
-noeq type member_info (bytes:Type0) {|crypto_bytes bytes|} = {
+type member_info (bytes:Type0) {|crypto_bytes bytes|} = {
   public_key: hpke_public_key bytes;
   version: nat;
 }
 
 //TODO: move this in Crypto.fsti?
-noeq type path_secret_ciphertext (bytes:Type0) {|crypto_bytes bytes|} = {
+type path_secret_ciphertext (bytes:Type0) {|crypto_bytes bytes|} = {
   kem_output: hpke_kem_output bytes;
   ciphertext: bytes;
 }
 
 type direction = | Left | Right
 
-noeq type key_package (bytes:Type0) {|crypto_bytes bytes|} = {
+type key_package (bytes:Type0) {|crypto_bytes bytes|} = {
   public_key: hpke_public_key bytes;
   version: nat;
   last_group_context: bytes; //Related to version, correspond to the info used in the ciphertexts
@@ -28,5 +28,7 @@ noeq type key_package (bytes:Type0) {|crypto_bytes bytes|} = {
   path_secret_ciphertext: list (path_secret_ciphertext bytes);
 }
 
-type treekem (bytes:Type0) {|crypto_bytes bytes|} (l:nat) (i:tree_index l) = tree l i (option (member_info bytes)) (option (key_package bytes))
-type pathkem (bytes:Type0) {|crypto_bytes bytes|} (l:nat) (i:tree_index l) (li:leaf_index l i) = path l i li (member_info bytes) (option (key_package bytes))
+let treekem (bytes:Type0) {|crypto_bytes bytes|} =
+  tree (option (member_info bytes)) (option (key_package bytes))
+let pathkem (bytes:Type0) {|crypto_bytes bytes|} =
+  path (member_info bytes) (option (key_package bytes))
