fstar/MLS.TreeSync.Extensions.fst
@@ -1,7 +1,6 @@
 module MLS.TreeSync.Extensions
 
 open Comparse
-open Lib.LoopCombinators
 open MLS.NetworkTypes
 open MLS.Result
 
@@ -16,9 +15,6 @@ type application_id_ext_nt (bytes:Type0) {|bytes_like bytes|} = {
 %splice [ps_application_id_ext_nt] (gen_parser (`application_id_ext_nt))
 
 (*** Utility functions ***)
-
-val ps_extensions: #bytes:Type0 -> {|bytes_like bytes|} -> parser_serializer bytes (mls_list bytes ps_extension_nt)
-let ps_extensions #bytes #bl = ps_mls_list ps_extension_nt
 
 #push-options "--ifuel 1 --fuel 1"
 val find_extension_index: #bytes:Type0 -> {|bytes_like bytes|} -> extension_type_nt -> extensions:list (extension_nt bytes) -> option (i:nat{i < List.length extensions})
@@ -35,18 +31,14 @@ let rec find_extension_index t extensions =
     )
 #pop-options
 
-val get_extension: #bytes:Type0 -> {|bytes_like bytes|} -> extension_type_nt -> bytes -> option bytes
-let get_extension #bytes #bl t extensions_buf =
-  match (ps_to_pse ps_extensions).parse_exact extensions_buf with
+val get_extension: #bytes:Type0 -> {|bytes_like bytes|} -> extension_type_nt -> list (extension_nt bytes) -> option bytes
+let get_extension #bytes #bl t extensions =
+  match find_extension_index t extensions with
   | None -> None
-  | Some extensions ->
-    match find_extension_index t extensions with
-    | None -> None
-    | Some i -> Some ((List.Tot.index extensions i).extension_data)
+  | Some i -> Some ((List.Tot.index extensions i).extension_data)
 
-val set_extension: #bytes:Type0 -> {|bytes_like bytes|} -> extension_type_nt -> bytes -> bytes -> result bytes
-let set_extension #bytes #bl t extensions_buf data =
-  extensions <-- from_option "set_extension: invalid extensions buffer" ((ps_to_pse ps_extensions).parse_exact extensions_buf);
+val set_extension: #bytes:Type0 -> {|bytes_like bytes|} -> extension_type_nt -> list (extension_nt bytes) -> bytes -> result (mls_list bytes ps_extension_nt )
+let set_extension #bytes #bl t extensions data =
   if not (length data < pow2 30) then
     error "set_extension: data is too long"
   else (
@@ -59,40 +51,35 @@ let set_extension #bytes #bl t extensions_buf data =
         ext_before @ [ext] @ ext_after
       )
     in
-    let ext_byte_length = bytes_length ps_extension_nt new_extensions in
-    if not (ext_byte_length < pow2 30) then
-      error "set_extension: new extension buffer is too long"
-    else (
-      return ((ps_to_pse ps_extensions).serialize_exact new_extensions)
-    )
+    if not (bytes_length #bytes ps_extension_nt new_extensions < pow2 30) then
+      error "set_extension: new_extensions too long"
+    else
+      return new_extensions
   )
 
-val mk_get_extension: #bytes:Type0 -> {|bytes_like bytes|} -> #a:Type0 -> extension_type_nt -> parser_serializer bytes a -> bytes -> option a
-let mk_get_extension #bytes #bl #a ext_type ps_a buf =
-  match get_extension ext_type buf with
+val mk_get_extension: #bytes:Type0 -> {|bytes_like bytes|} -> #a:Type0 -> extension_type_nt -> parser_serializer bytes a -> list (extension_nt bytes) -> option a
+let mk_get_extension #bytes #bl #a ext_type ps_a extensions =
+  match get_extension ext_type extensions with
   | None -> None
   | Some res ->
     (ps_to_pse ps_a).parse_exact res
 
-val mk_set_extension: #bytes:Type0 -> {|bytes_like bytes|} -> #a:Type0 -> extension_type_nt -> parser_serializer bytes a -> bytes -> a -> result bytes
-let mk_set_extension #a ext_type ps_a buf ext_content =
-  set_extension ext_type buf ((ps_to_pse ps_a).serialize_exact ext_content)
+val mk_set_extension: #bytes:Type0 -> {|bytes_like bytes|} -> #a:Type0 -> extension_type_nt -> parser_serializer bytes a -> list (extension_nt bytes) -> a -> result (mls_list bytes ps_extension_nt)
+let mk_set_extension #a ext_type ps_a extensions ext_content =
+  set_extension ext_type extensions ((ps_to_pse ps_a).serialize_exact ext_content)
 
 (*** Exposed functions ***)
 
-#push-options "--fuel 1"
-val empty_extensions: #bytes:Type0 -> {|bytes_like bytes|} -> bytes
+val empty_extensions: #bytes:Type0 -> {|bytes_like bytes|} -> mls_list bytes ps_extension_nt
 let empty_extensions #bytes #bl =
   bytes_length_nil #bytes ps_extension_nt;
-  (ps_to_pse ps_extensions).serialize_exact []
-#pop-options
+  []
 
-val get_extension_list: #bytes:Type0 -> {|bytes_like bytes|} -> bytes -> result (list (extension_type_nt))
-let get_extension_list #bytes #bl extensions_buf =
-  extensions <-- from_option "set_extension: invalid extensions buffer" ((ps_to_pse ps_extensions).parse_exact extensions_buf);
-  return (List.Tot.map (fun x -> x.extension_type) extensions)
+val get_extension_list: #bytes:Type0 -> {|bytes_like bytes|} -> list (extension_nt bytes) -> list (extension_type_nt)
+let get_extension_list #bytes #bl extensions =
+  (List.Tot.map (fun x -> x.extension_type) extensions)
 
-val get_application_id_extension: #bytes:Type0 -> {|bytes_like bytes|} -> bytes -> option (application_id_ext_nt bytes)
+val get_application_id_extension: #bytes:Type0 -> {|bytes_like bytes|} -> list (extension_nt bytes) -> option (application_id_ext_nt bytes)
 let get_application_id_extension #bytes #bl = mk_get_extension (ET_application_id ()) ps_application_id_ext_nt
-val set_application_id_extension: #bytes:Type0 -> {|bytes_like bytes|} -> bytes -> application_id_ext_nt bytes -> result bytes
+val set_application_id_extension: #bytes:Type0 -> {|bytes_like bytes|} -> list (extension_nt bytes) -> application_id_ext_nt bytes -> result (mls_list bytes ps_extension_nt)
 let set_application_id_extension #bytes #bl = mk_set_extension (ET_application_id ()) ps_application_id_ext_nt
