fstar/MLS.TreeSync.ParentHash.fst
@@ -1,6 +1,7 @@
 module MLS.TreeSync.ParentHash
 
 open Comparse
+open MLS.TreeSync.NetworkTypes
 open MLS.TreeSync.Types
 open MLS.TreeSync.Hash
 open MLS.Crypto
@@ -10,29 +11,23 @@ open MLS.Result
 
 #set-options "--ifuel 1 --fuel 1"
 
-noeq type parent_hash_input_nt (bytes:Type0) {|bytes_like bytes|} = {
-  encryption_key: hpke_public_key_nt bytes;
+noeq type parent_hash_input_nt (bytes:Type0) {|bytes_like bytes|} (tkt:treekem_types bytes) = {
+  [@@@ with_parser tkt.ps_node_content]
+  content: tkt.node_content; //encryption_key
   parent_hash: mls_bytes bytes;
   original_sibling_tree_hash: mls_bytes bytes;
 }
 
 %splice [ps_parent_hash_input_nt] (gen_parser (`parent_hash_input_nt))
 
-instance parseable_serializeable_parent_hash_input_nt (bytes:Type0) {|bytes_like bytes|}: parseable_serializeable bytes (parent_hash_input_nt bytes) =
-  mk_parseable_serializeable ps_parent_hash_input_nt
+instance parseable_serializeable_parent_hash_input_nt (bytes:Type0) {|bytes_like bytes|} (tkt:treekem_types bytes): parseable_serializeable bytes (parent_hash_input_nt bytes tkt) =
+  mk_parseable_serializeable (ps_parent_hash_input_nt tkt)
 
-val get_encryption_key_from_content: #bytes:Type0 -> {|bytes_like bytes|} -> bytes -> result (hpke_public_key_nt bytes)
-let get_encryption_key_from_content #bytes #bl content =
-  let open MLS.NetworkBinder in
-  content <-- from_option "get_encryption_key_from_content: Couldn't parse node content"
-    (parse (treekem_content_nt bytes) content);
-  return content.encryption_key
-
-val un_add: #bytes:Type0 -> {|bytes_like bytes|} -> #l:nat -> #i:tree_index l -> treesync bytes l i -> list nat -> treesync bytes l i
-let rec un_add #bytes #bl #l #i t leaves =
+val un_add: #bytes:Type0 -> {|bytes_like bytes|} -> #tkt:treekem_types bytes -> #l:nat -> #i:tree_index l -> treesync bytes tkt l i -> list (nat_lbytes 4) -> treesync bytes tkt l i
+let rec un_add #bytes #bl #tkt #l #i t leaves =
   match t with
   | TLeaf olp -> (
-    if List.Tot.mem i leaves then
+    if i < pow2 32 && List.Tot.mem i leaves then
       TLeaf None
     else
       TLeaf olp
@@ -43,7 +38,9 @@ let rec un_add #bytes #bl #l #i t leaves =
       | None -> None
       | Some np -> (
         let new_unmerged_leaves = List.Tot.filter (fun l -> not (List.Tot.mem l leaves)) np.unmerged_leaves in
-        Some ({ np with unmerged_leaves = new_unmerged_leaves } <: node_package_t bytes)
+        //TODO: remove assume by proving it
+        assume(bytes_length #bytes (ps_nat_lbytes 4) new_unmerged_leaves < pow2 30);
+        Some ({ np with unmerged_leaves = new_unmerged_leaves } <: parent_node_nt bytes tkt)
       )
     in
     let new_left = un_add left leaves in
@@ -51,12 +48,11 @@ let rec un_add #bytes #bl #l #i t leaves =
     TNode new_onp new_left new_right
 
 //Note: We could remove the `result` (i.e. prove that the hash input doesn't exceed pow2 61 + add precondition).
-val compute_parent_hash: #bytes:Type0 -> {|crypto_bytes bytes|} -> #l:nat -> #i:tree_index l -> bytes -> mls_bytes bytes -> treesync bytes l i -> result (mls_bytes bytes)
-let compute_parent_hash #bytes #cb #l #i kem_content parent_hash sibling =
-  encryption_key <-- get_encryption_key_from_content kem_content;
+val compute_parent_hash: #bytes:Type0 -> {|crypto_bytes bytes|} -> #tkt:treekem_types bytes -> #l:nat -> #i:tree_index l -> tkt.node_content -> mls_bytes bytes -> treesync bytes tkt l i -> result (mls_bytes bytes)
+let compute_parent_hash #bytes #cb #tkt #l #i kem_content parent_hash sibling =
   original_sibling_tree_hash <-- tree_hash sibling;
-  res <-- hash_hash #bytes (serialize (parent_hash_input_nt bytes) ({
-    encryption_key;
+  res <-- hash_hash #bytes (serialize (parent_hash_input_nt bytes tkt) ({
+    content = kem_content;
     parent_hash = parent_hash;
     original_sibling_tree_hash;
   }));
