fstar/MLS.TreeSync.Types.fst
@@ -7,70 +7,27 @@ open MLS.Tree
 
 #set-options "--fuel 1 --ifuel 1"
 
-(** Identity and Credentials *)
-type credential_t (bytes:Type0) {|bytes_like bytes|} = {
-  version: nat; //For security proofs, should be erasable
-  identity: bytes;
-  signature_key: bytes;
-}
-
-(** Secrets belonging to a Group member  *)
-noeq type leaf_secrets_t (bytes:Type0) {|bytes_like bytes|} = {
-  identity_sig_key: bytes;
-}
-
-type external_content (bytes:Type0) {|bytes_like bytes|} = {
-  content: bytes; //Roughly, data sent on the wire
-  impl_data: bytes; //Roughly, internal data specific to the implementation details
-}
-
-(** Definition of a Leaf package *)
-type leaf_package_t (bytes:Type0) {|bytes_like bytes|} = {
-  version: nat; //For security proofs, should be erasable
-  content: external_content bytes;
-  credential: credential_t bytes;
-  capabilities: capabilities_nt bytes;
-  source: leaf_node_source_nt;
-  lifetime: leaf_node_lifetime_nt source;
-  parent_hash: leaf_node_parent_hash_nt bytes source;
-  extensions: bytes;
-  signature: bytes;
-}
-
-(** Definition of a Node package *)
-type node_package_t (bytes:Type0) {|bytes_like bytes|} = {
-  version: nat; //For security proofs, should be erasable
-  unmerged_leaves: list nat;
-  parent_hash: mls_bytes bytes;
-  content: external_content bytes;
-}
-
 (** Tree and Paths definitions *)
-type treesync (bytes:Type0) {|bytes_like bytes|} (l:nat) (i:tree_index l) = tree l i (option (leaf_package_t bytes)) (option (node_package_t bytes))
+let treesync (bytes:Type0) {|bytes_like bytes|} (tkt:treekem_types bytes) =
+  tree (option (leaf_node_nt bytes tkt)) (option (parent_node_nt bytes tkt))
 
-type external_pathsync (bytes:Type0) {|bytes_like bytes|} (l:nat) (i:tree_index l) (li:leaf_index l i) = path l i li (leaf_package_t bytes) (option (external_content bytes))
-
-type operation_t (bytes:Type0) {|bytes_like bytes|} =
-  | Op_Add: lp:leaf_package_t bytes -> operation_t bytes
-  | Op_Update: lp:leaf_package_t bytes -> operation_t bytes
-  | Op_Remove: ind:nat -> operation_t bytes
-  | Op_UpdatePath: l:nat -> i:tree_index l -> li:leaf_index l i -> external_pathsync bytes l i li -> operation_t bytes
+let external_pathsync (bytes:Type0) {|bytes_like bytes|} (tkt:treekem_types bytes) =
+  path (leaf_node_nt bytes tkt) (option tkt.node_content)
 
 (** TreeSync state and accessors *)
-type state_t (bytes:Type0) {|bytes_like bytes|} = {
+noeq type state_t (bytes:Type0) {|bytes_like bytes|} (tkt:treekem_types bytes) = {
   group_id: bytes;
   levels: nat;
-  tree: treesync bytes levels 0;
+  tree: treesync bytes tkt levels 0;
   version: nat;
-  //initial_tree: treesync levels treesize;
-  transcript: Seq.seq (operation_t bytes);
 }
 
-val mk_initial_state: #bytes:Type0 -> {|bytes_like bytes|} -> gid:bytes -> l:nat -> treesync bytes l 0 -> state_t bytes
+val mk_initial_state: #bytes:Type0 -> {|bytes_like bytes|} -> #tkt:treekem_types bytes -> gid:bytes -> l:nat -> treesync bytes tkt l 0 -> state_t bytes tkt
 let mk_initial_state gid l t = {
-  group_id = gid; levels = l;
-  tree = t; version = 0;
-  //initial_tree = t;
-  transcript = Seq.empty;}
+  group_id = gid;
+  levels = l;
+  tree = t;
+  version = 0;
+}
 
-type index_t (#bytes:Type0) {|bytes_like bytes|} (st:state_t bytes) = i:nat{i < pow2 st.levels}
+type index_t (#bytes:Type0) {|bytes_like bytes|} (#tkt:treekem_types bytes) (st:state_t bytes tkt) = i:nat{i < pow2 st.levels}
