fstar/MLS.TreeSync.fst
@@ -4,80 +4,63 @@ open Comparse
 open MLS.Crypto
 open MLS.NetworkTypes
 open MLS.TreeSync.NetworkTypes
-open MLS.NetworkBinder
-open MLS.Utils
 open MLS.Tree
+open MLS.TreeCommon
 open MLS.TreeSync.Types
 open MLS.TreeSync.ParentHash
 open MLS.Result
 
 #set-options "--fuel 1 --ifuel 1"
 
-(*** Tree creation ***)
-
-val create_tree: #bytes:Type0 -> {|bytes_like bytes|} -> leaf_package_t bytes -> treesync bytes 0 0
-let create_tree lp =
-  TLeaf (Some lp)
-
 (*** Tree operations ***)
 
-val tree_add: #bytes:Type0 -> {|bytes_like bytes|} -> #l:nat -> #i:tree_index l -> treesync bytes l i -> li:leaf_index l i -> leaf_package_t bytes -> treesync bytes l i
-let rec tree_add #bytes #bl #l #i t li lp =
+val tree_add: #bytes:Type0 -> {|bytes_like bytes|} -> #tkt:treekem_types bytes -> #l:nat -> #i:tree_index l -> treesync bytes tkt l i -> li:leaf_index l i -> leaf_node_nt bytes tkt -> result (treesync bytes tkt l i)
+let rec tree_add #bytes #bl #tkt #l #i t li lp =
   match t with
-  | TLeaf _ -> TLeaf (Some lp)
+  | TLeaf _ -> return (TLeaf (Some lp))
   | TNode opt_content left right -> (
-    let new_opt_content =
+    new_opt_content <-- (
       match opt_content with
-      | None -> None
-      | Some content -> Some ({
-        content with unmerged_leaves = insert_sorted li content.unmerged_leaves
-      })
-    in
-    if is_left_leaf li
-    then TNode new_opt_content (tree_add left li lp) right
-    else TNode new_opt_content left (tree_add right li lp)
-   )
-
-val tree_blank_path: #bytes:Type0 -> {|bytes_like bytes|} -> #l:nat -> #i:tree_index l -> treesync bytes l i -> leaf_index l i -> option (leaf_package_t bytes) -> treesync bytes l i
-let rec tree_blank_path #bytes #bl #l #i t li opt_lp =
-  match t with
-  | TLeaf _ -> TLeaf opt_lp
-  | TNode opt_node_content left right -> (
-    if is_left_leaf li
-    then TNode None (tree_blank_path left li opt_lp) right
-    else TNode None left (tree_blank_path right li opt_lp)
+      | None -> return None
+      | Some content -> (
+        if not (li < pow2 32) then
+          error ""
+        else if not (bytes_length #bytes (ps_nat_lbytes 4) (insert_sorted li content.unmerged_leaves) < pow2 30) then
+          error ""
+        else
+          return (Some ({content with unmerged_leaves = insert_sorted li content.unmerged_leaves}))
+      )
+    );
+    if is_left_leaf li then (
+      new_left <-- (tree_add left li lp);
+      return (TNode new_opt_content new_left right)
+    ) else (
+      new_right <-- (tree_add right li lp);
+      return (TNode new_opt_content left new_right)
+    )
   )
 
-val tree_update: #bytes:Type0 -> {|bytes_like bytes|} -> #l:nat -> #i:tree_index l -> treesync bytes l i -> leaf_index l i -> leaf_package_t bytes -> treesync bytes l i
-let tree_update #bytes #bl #l #i t li lp =
-  tree_blank_path t li (Some lp)
-
-val tree_remove: #bytes:Type0 -> {|bytes_like bytes|} -> #l:nat -> #i:tree_index l -> treesync bytes l i -> leaf_index l i -> treesync bytes l i
-let tree_remove #bytes #bl #l #i t li =
-  tree_blank_path t li None
-
-val compute_new_np_and_ph: #bytes:Type0 -> {|crypto_bytes bytes|} -> #l:nat -> #i:tree_index l -> option (external_content bytes) -> treesync bytes l i -> mls_bytes bytes -> result (option (node_package_t bytes) & mls_bytes bytes)
-let compute_new_np_and_ph #bytes #cb #l #i opt_ext_content sibling parent_parent_hash =
+val compute_new_np_and_ph: #bytes:Type0 -> {|crypto_bytes bytes|} -> #tkt:treekem_types bytes -> #l:nat -> #i:tree_index l -> option (tkt.node_content) -> treesync bytes tkt l i -> mls_bytes bytes -> result (option (parent_node_nt bytes tkt) & mls_bytes bytes)
+let compute_new_np_and_ph #bytes #cb #tkt #l #i opt_ext_content sibling parent_parent_hash =
   let new_opt_content =
     match opt_ext_content with
     | Some ext_content -> Some ({
-      version = 0;
-      unmerged_leaves = [];
-      parent_hash = parent_parent_hash;
       content = ext_content;
-    } <: node_package_t bytes)
+      parent_hash = parent_parent_hash;
+      unmerged_leaves = (bytes_length_nil #bytes (ps_nat_lbytes 4); []);
+    } <: parent_node_nt bytes tkt)
     | None -> None
   in
   new_parent_parent_hash <-- (
     match opt_ext_content with
     | Some ext_content ->
-      compute_parent_hash ext_content.content parent_parent_hash sibling
+      compute_parent_hash ext_content parent_parent_hash sibling
     | None -> return parent_parent_hash
   );
   return (new_opt_content, new_parent_parent_hash)
 
-val compute_leaf_parent_hash_from_external_path: #bytes:Type0 -> {|crypto_bytes bytes|} -> #l:nat -> #i:tree_index l -> #li:leaf_index l i -> t:treesync bytes l i -> external_pathsync bytes l i li -> mls_bytes bytes -> result (mls_bytes bytes)
-let rec compute_leaf_parent_hash_from_external_path #bytes #cb #l #i #li t p parent_parent_hash =
+val compute_leaf_parent_hash_from_external_path: #bytes:Type0 -> {|crypto_bytes bytes|} -> #tkt:treekem_types bytes -> #l:nat -> #i:tree_index l -> #li:leaf_index l i -> t:treesync bytes tkt l i -> external_pathsync bytes tkt l i li -> mls_bytes bytes -> result (mls_bytes bytes)
+let rec compute_leaf_parent_hash_from_external_path #bytes #cb #tkt #l #i #li t p parent_parent_hash =
   match t, p with
   | TLeaf old_lp, PLeaf new_lp -> (
     return parent_parent_hash
@@ -91,69 +74,68 @@ let rec compute_leaf_parent_hash_from_external_path #bytes #cb #l #i #li t p par
     else
       compute_leaf_parent_hash_from_external_path right p_next new_parent_parent_hash
 
-val get_external_path_leaf: #bytes:Type0 -> {|crypto_bytes bytes|} -> #l:nat -> #i:tree_index l -> #li:leaf_index l i -> external_pathsync bytes l i li -> leaf_package_t bytes
-let rec get_external_path_leaf #bytes #cb #l #i #li p =
+val get_external_path_leaf: #bytes:Type0 -> {|crypto_bytes bytes|} -> #tkt:treekem_types bytes -> #l:nat -> #i:tree_index l -> #li:leaf_index l i -> external_pathsync bytes tkt l i li -> leaf_node_nt bytes tkt
+let rec get_external_path_leaf #bytes #cb #tkt #l #i #li p =
   match p with
   | PLeaf lp -> lp
   | PNode _ p_next -> get_external_path_leaf p_next
 
-val set_external_path_leaf: #bytes:Type0 -> {|crypto_bytes bytes|} -> #l:nat -> #i:tree_index l -> #li:leaf_index l i -> external_pathsync bytes l i li -> leaf_package_t bytes -> external_pathsync bytes l i li
-let rec set_external_path_leaf #bytes #cb #l #i #li p lp =
+val set_external_path_leaf: #bytes:Type0 -> {|crypto_bytes bytes|} -> #tkt:treekem_types bytes -> #l:nat -> #i:tree_index l -> #li:leaf_index l i -> external_pathsync bytes tkt l i li -> leaf_node_nt bytes tkt -> external_pathsync bytes tkt l i li
+let rec set_external_path_leaf #bytes #cb #tkt #l #i #li p lp =
   match p with
   | PLeaf _ -> PLeaf lp
   | PNode p_content p_next -> PNode p_content (set_external_path_leaf p_next lp)
 
-val get_leaf_package_tbs: #bytes:Type0 -> {|bytes_like bytes|} -> leaf_package_t bytes -> bytes -> result bytes
-let get_leaf_package_tbs #bytes #bl lp group_id =
-    ln <-- leaf_package_to_network lp;
+val get_leaf_package_tbs: #bytes:Type0 -> {|bytes_like bytes|} -> #tkt:treekem_types bytes -> leaf_node_data_nt bytes tkt -> bytes -> result bytes
+let get_leaf_package_tbs #bytes #bl #tkt lp_data group_id =
     if not (length group_id < pow2 30) then
       internal_failure "sign_leaf: group_id is too long"
     else (
       let ln_tbs = ({
-        data = ln.data;
-        group_id = (match ln.data.source with |LNS_update () |LNS_commit() -> group_id |_ -> ());
-      } <: leaf_node_tbs_nt bytes MLS.TreeKEM.NetworkTypes.tkt) in
+        data = lp_data;
+        group_id = (match lp_data.source with |LNS_update () |LNS_commit() -> group_id |_ -> ());
+      } <: leaf_node_tbs_nt bytes tkt) in
       return (serialize (leaf_node_tbs_nt bytes _) ln_tbs)
     )
 
-val external_path_is_valid: #bytes:Type0 -> {|crypto_bytes bytes|} -> #l:nat -> #i:tree_index l -> #li:leaf_index l i -> t:treesync bytes l i -> external_pathsync bytes l i li -> bytes -> result bool
-let external_path_is_valid #bytes #cb #l #i #li t p group_id =
+val external_path_is_valid: #bytes:Type0 -> {|crypto_bytes bytes|} -> #tkt:treekem_types bytes -> #l:nat -> #i:tree_index l -> #li:leaf_index l i -> t:treesync bytes tkt l i -> external_pathsync bytes tkt l i li -> bytes -> result bool
+let external_path_is_valid #bytes #cb #tkt #l #i #li t p group_id =
   let old_lp = leaf_at t li in
   let new_lp = get_external_path_leaf p in
   //TODO: something stating that new_lp is related to old_lp
   computed_parent_hash <-- compute_leaf_parent_hash_from_external_path t p root_parent_hash;
-  tbs <-- get_leaf_package_tbs new_lp group_id;
+  tbs <-- get_leaf_package_tbs new_lp.data group_id;
   verification_key <-- (
-    if not (length new_lp.credential.signature_key = sign_public_key_length #bytes) then
+    if not (length #bytes new_lp.data.signature_key = sign_public_key_length #bytes) then
       error "external_path_is_valid: verification key has wrong length"
     else
-      return (new_lp.credential.signature_key <: sign_public_key bytes)
+      return (new_lp.data.signature_key <: sign_public_key bytes)
   );
   signature <-- (
-    if not (length new_lp.signature = sign_signature_length #bytes) then
+    if not (length #bytes new_lp.signature = sign_signature_length #bytes) then
       error "external_path_is_valid: signature has wrong length"
     else
       return (new_lp.signature <: sign_signature bytes)
   );
   signature_ok <-- verify_with_label verification_key (string_to_bytes #bytes "LeafNodeTBS") tbs signature;
-  let parent_hash_ok = (new_lp.source = LNS_commit () && (new_lp.parent_hash <: bytes) = computed_parent_hash) in
+  let parent_hash_ok = (new_lp.data.source = LNS_commit () && (new_lp.data.parent_hash <: bytes) = computed_parent_hash) in
   return (signature_ok && parent_hash_ok)
 
-val external_path_to_valid_external_path: #bytes:Type0 -> {|crypto_bytes bytes|} -> #l:nat -> #i:tree_index l -> #li:leaf_index l i -> t:treesync bytes l i -> external_pathsync bytes l i li -> bytes -> sign_private_key bytes -> sign_nonce bytes -> result (external_pathsync bytes l i li)
-let external_path_to_valid_external_path #bytes #cb #l #i #li t p group_id sign_key nonce =
+val external_path_to_valid_external_path: #bytes:Type0 -> {|crypto_bytes bytes|} -> #tkt:treekem_types bytes -> #l:nat -> #i:tree_index l -> #li:leaf_index l i -> t:treesync bytes tkt l i -> external_pathsync bytes tkt l i li -> bytes -> sign_private_key bytes -> sign_nonce bytes -> result (external_pathsync bytes tkt l i li)
+let external_path_to_valid_external_path #bytes #cb #tkt #l #i #li t p group_id sign_key nonce =
   computed_parent_hash <-- compute_leaf_parent_hash_from_external_path t p root_parent_hash;
   let lp = get_external_path_leaf p in
-  if not (lp.source = LNS_commit ()) then
+  if not (lp.data.source = LNS_commit ()) then
     error "external_path_to_valid_external_path: source is not a commit"
   else (
-    let new_lp = { lp with parent_hash = computed_parent_hash; } in
-    new_lp_tbs <-- get_leaf_package_tbs new_lp group_id;
+    let new_lp_data = { lp.data with parent_hash = computed_parent_hash; } in
+    new_lp_tbs <-- get_leaf_package_tbs new_lp_data group_id;
     new_signature <-- sign_with_label sign_key (string_to_bytes #bytes "LeafNodeTBS") new_lp_tbs nonce;
-    return (set_external_path_leaf p ({ new_lp with signature = new_signature }))
+    return (set_external_path_leaf p ({ data = new_lp_data; signature = new_signature }))
   )
 
-val apply_external_path_aux: #bytes:Type0 -> {|crypto_bytes bytes|} -> #l:nat -> #i:tree_index l -> #li:leaf_index l i -> t:treesync bytes l i -> external_pathsync bytes l i li -> mls_bytes bytes -> result (treesync bytes l i)
-let rec apply_external_path_aux #bytes #cb #l #i #li t p parent_parent_hash =
+val apply_external_path_aux: #bytes:Type0 -> {|crypto_bytes bytes|} -> #tkt:treekem_types bytes -> #l:nat -> #i:tree_index l -> #li:leaf_index l i -> t:treesync bytes tkt l i -> external_pathsync bytes tkt l i li -> mls_bytes bytes -> result (treesync bytes tkt l i)
+let rec apply_external_path_aux #bytes #cb #tkt #l #i #li t p parent_parent_hash =
   match t, p with
   | TLeaf _, PLeaf lp -> return (TLeaf (Some lp))
   | TNode _ left right, PNode opt_ext_content p_next ->
@@ -168,97 +150,57 @@ let rec apply_external_path_aux #bytes #cb #l #i #li t p parent_parent_hash =
       return (TNode new_opt_content left new_right)
     )
 
-val apply_external_path: #bytes:Type0 -> {|crypto_bytes bytes|} -> #l:nat -> #i:tree_index l -> #li:leaf_index l i -> t:treesync bytes l i -> external_pathsync bytes l i li -> result (treesync bytes l i)
-let apply_external_path #bytes #cb #l #i #li t p =
+val apply_external_path: #bytes:Type0 -> {|crypto_bytes bytes|} -> #tkt:treekem_types bytes -> #l:nat -> #i:tree_index l -> #li:leaf_index l i -> t:treesync bytes tkt l i -> external_pathsync bytes tkt l i li -> result (treesync bytes tkt l i)
+let apply_external_path #bytes #cb #tkt #l #i #li t p =
   apply_external_path_aux t p root_parent_hash
-
-(*** Tree extension / truncation ***)
-
-val is_tree_empty: #bytes:Type0 -> {|bytes_like bytes|} -> #l:nat -> #i:tree_index l -> treesync bytes l i -> bool
-let rec is_tree_empty #bytes #bl #l #i t =
-  match t with
-  | TNode _ left right ->
-    is_tree_empty left && is_tree_empty right
-  | TLeaf (Some _) -> false
-  | TLeaf None -> true
-
-val canonicalize_tree: #bytes:Type0 -> {|bytes_like bytes|} -> #l:nat -> treesync bytes l 0 -> (l_res:nat{l_res <= l} & treesync bytes l_res 0)
-let canonicalize_tree #bytes #bl #l t0 =
-  match t0 with
-  | TLeaf _ -> (|_, t0|)
-  | TNode _ left right ->
-    if is_tree_empty right then (|_, left|)
-    else (|_, t0|)
-
-// Helper functions to add leaf / extend the tree
-
-val find_empty_leaf: #bytes:Type0 -> {|bytes_like bytes|} -> #l:nat -> #i:tree_index l -> treesync bytes l i -> option (leaf_index l i)
-let rec find_empty_leaf #bytes #bl #l #i t =
-  match t with
-  | TLeaf (Some _) -> None
-  | TLeaf None -> Some i
-  | TNode _ left right -> (
-    match find_empty_leaf left, find_empty_leaf right with
-    | Some x, _ -> Some x
-    | None, Some x -> Some x
-    | None, None -> None
-  )
-
-val mk_blank_tree: #bytes:Type0 -> {|bytes_like bytes|} -> l:nat -> i:tree_index l -> Pure (treesync bytes l i) (requires True) (ensures fun res -> Some? (find_empty_leaf res))
-let rec mk_blank_tree #bytes #bl l i =
-  if l = 0 then TLeaf None
-  else TNode None (mk_blank_tree (l-1) _) (mk_blank_tree (l-1) _)
-
-val add_one_level: #bytes:Type0 -> {|bytes_like bytes|} -> #l:nat -> treesync bytes l 0 -> Pure (treesync bytes (l+1) 0) (requires True) (fun res -> Some? (find_empty_leaf res))
-let add_one_level #bytes #bl #l t =
-  TNode None t (mk_blank_tree l _)
 
 (*** Higher-level API ***)
 
-open MLS.NetworkTypes
-open MLS.NetworkBinder
-open MLS.Crypto
-open MLS.Result
-
-val create: #bytes:Type0 -> {|bytes_like bytes|} -> gid:bytes -> leaf_package_t bytes -> state_t bytes
+val create: #bytes:Type0 -> {|bytes_like bytes|} -> #tkt:treekem_types bytes -> gid:bytes -> leaf_node_nt bytes tkt -> state_t bytes tkt
 let create #bytes #bl gid lp =
   mk_initial_state gid 0 (create_tree lp)
 
-val state_update_tree: #bytes:Type0 -> {|bytes_like bytes|} -> #l:nat -> state_t bytes -> treesync bytes l 0 -> state_t bytes
-let state_update_tree #bytes #bl #l st new_tree =
+val state_update_tree: #bytes:Type0 -> {|bytes_like bytes|} -> #tkt:treekem_types bytes -> #l:nat -> state_t bytes tkt -> treesync bytes tkt l 0 -> state_t bytes tkt
+let state_update_tree #bytes #bl #tkt #l st new_tree =
   ({ st with
     levels = l;
     version = st.version + 1;
     tree = new_tree;
-    //transcript = Seq.snoc st.transcript op //TODO
   })
 
-val get_leaf_package_from_key_package: #bytes:Type0 -> {|crypto_bytes bytes|} -> key_package_nt bytes MLS.TreeKEM.NetworkTypes.tkt -> result (leaf_package_t bytes)
+val get_leaf_package_from_key_package: #bytes:Type0 -> {|crypto_bytes bytes|} -> #tkt:treekem_types bytes -> key_package_nt bytes tkt -> result (leaf_node_nt bytes tkt)
 let get_leaf_package_from_key_package #bytes #cb kp =
   //TODO check signature
   if not (kp.tbs.leaf_node.data.source = LNS_key_package ()) then
     error "get_leaf_package_from_key_package: source is not add"
   else (
-    network_to_leaf_package kp.tbs.leaf_node
+    return kp.tbs.leaf_node
   )
 
-val add: #bytes:Type0 -> {|crypto_bytes bytes|} -> state_t bytes -> key_package_nt bytes MLS.TreeKEM.NetworkTypes.tkt -> result (state_t bytes & nat)
-let add #bytes #bl st kp =
+val add: #bytes:Type0 -> {|crypto_bytes bytes|} -> #tkt:treekem_types bytes -> state_t bytes tkt -> key_package_nt bytes tkt -> result (state_t bytes tkt & nat)
+let add #bytes #bl #tkt st kp =
   lp <-- get_leaf_package_from_key_package kp;
   match find_empty_leaf st.tree with
   | Some i ->
-    return (state_update_tree st (tree_add st.tree i lp), (i <: nat))
+    new_tree <-- tree_add st.tree i lp;
+    return (state_update_tree st new_tree, (i <: nat))
   | None ->
     let augmented_tree = add_one_level st.tree in
     let i = Some?.v (find_empty_leaf augmented_tree) in
-    return (state_update_tree st (tree_add augmented_tree i lp), i)
+    new_tree <-- tree_add augmented_tree i lp;
+    return (state_update_tree st new_tree, (i <: nat))
 
-val update: #bytes:Type0 -> {|bytes_like bytes|} -> st:state_t bytes -> leaf_package_t bytes -> index_t st -> state_t bytes
-let update #bytes #bl st lp i =
+val update: #bytes:Type0 -> {|bytes_like bytes|} -> #tkt:treekem_types bytes -> st:state_t bytes tkt -> leaf_node_nt bytes tkt -> index_t st -> state_t bytes tkt
+let update #bytes #bl #tkt st lp i =
   state_update_tree st (tree_update st.tree i lp)
 
-val remove: #bytes:Type0 -> {|bytes_like bytes|} -> st:state_t bytes -> i:index_t st -> state_t bytes
-let remove #bytes #bl st i =
+val remove: #bytes:Type0 -> {|bytes_like bytes|} -> #tkt:treekem_types bytes -> st:state_t bytes tkt -> i:index_t st -> state_t bytes tkt
+let remove #bytes #bl #tkt st i =
   let blanked_tree = (tree_remove st.tree i) in
   let (|_, reduced_tree|) = canonicalize_tree blanked_tree in
   state_update_tree st reduced_tree
+
+val commit: #bytes:Type0 -> {|crypto_bytes bytes|} -> #tkt:treekem_types bytes -> st:state_t bytes tkt -> #li:index_t st -> external_pathsync bytes tkt st.levels 0 li -> result (state_t bytes tkt)
+let commit #bytes #cb #tkt st #li p =
+  new_tree <-- apply_external_path st.tree p;
+  return (state_update_tree st new_tree)
