fstar/MLS.TreeSyncTreeKEMBinder.fst
@@ -2,59 +2,42 @@ module MLS.TreeSyncTreeKEMBinder
 
 open Comparse
 open MLS.Crypto
-open MLS.NetworkTypes
 open MLS.TreeSync.NetworkTypes
 open MLS.TreeKEM.NetworkTypes
 open MLS.Tree
-open MLS.NetworkBinder
 open MLS.TreeSync.Types
 open MLS.TreeKEM.Types
 open MLS.Result
 
 #set-options "--fuel 1 --ifuel 1"
 
-val encrypted_path_secret_nt_to_tk: #bytes:Type0 -> {|crypto_bytes bytes|} -> hpke_ciphertext_nt bytes -> result (path_secret_ciphertext bytes)
-let encrypted_path_secret_nt_to_tk #bytes #cb x =
-  if not (length (x.kem_output <: bytes) = hpke_kem_output_length #bytes) then
-    internal_failure "encrypted_path_secret_nt_to_tk: kem_output has wrong length"
-  else
-    return ({
-      kem_output = x.kem_output;
-      ciphertext = x.ciphertext;
-    })
-
-val treesync_to_treekem_node_package: #bytes:Type0 -> {|crypto_bytes bytes|} -> node_package_t bytes -> result (key_package bytes)
+val treesync_to_treekem_node_package: #bytes:Type0 -> {|crypto_bytes bytes|} -> parent_node_nt bytes tkt -> result (key_package bytes)
 let treesync_to_treekem_node_package #bytes #cb np =
-  content <-- from_option "treesync_to_treekem_node_package: Couldn't parse node content"
-    (parse (treekem_content_nt bytes) np.content.content);
-  impl_data <-- from_option "treesync_to_treekem_node_package: Couldn't parse node impl data"
-    (parse (treekem_impl_data_nt bytes) np.content.impl_data);
-  path_secret_ciphertext <-- mapM (encrypted_path_secret_nt_to_tk #bytes) impl_data.encrypted_path_secret;
-  if not (length (content.encryption_key <: bytes) = hpke_public_key_length #bytes) then
+  if not (length (np.content <: bytes) = hpke_public_key_length #bytes) then
     error "treesync_to_treekem_node_package: public key has wrong length"
   else (
+    let unmerged_leaves = List.Tot.map #(nat_lbytes 4) #nat (fun x -> x) np.unmerged_leaves in
     return ({
-      public_key = content.encryption_key;
-      version = np.version;
-      last_group_context = impl_data.last_group_context;
-      unmerged_leaves = np.unmerged_leaves;
-      path_secret_from = impl_data.content_dir;
-      path_secret_ciphertext = path_secret_ciphertext;
+      public_key = np.content;
+      version = 0;
+      last_group_context = empty;
+      unmerged_leaves = unmerged_leaves;
+      path_secret_from = Left;
+      path_secret_ciphertext = [];
     })
   )
 
-val treesync_to_treekem: #bytes:Type0 -> {|crypto_bytes bytes|} -> #l:nat -> #i:tree_index l -> treesync bytes l i -> result (treekem bytes l i)
+// This does not contain any internal TreeKEM data. To be used then joining a new group.
+val treesync_to_treekem: #bytes:Type0 -> {|crypto_bytes bytes|} -> #l:nat -> #i:tree_index l -> treesync bytes tkt l i -> result (treekem bytes l i)
 let rec treesync_to_treekem #bytes #cb #l #i t =
   match t with
   | TLeaf None ->
     return (TLeaf None)
   | TLeaf (Some lp) ->
-    lpc <-- from_option "treesync_to_treekem: Couldn't parse leaf content"
-      (parse (treekem_content_nt bytes) lp.content.content);
-    if length (lpc.encryption_key <: bytes) = hpke_public_key_length #bytes then
-      return (TLeaf (Some ({public_key = lpc.encryption_key; version = lp.version} <: member_info bytes)))
-    else
+    if not (length (lp.data.content <: bytes) = hpke_public_key_length #bytes) then
       error "treesync_to_treekem: public key has wrong length"
+    else
+      return (TLeaf (Some ({public_key = lp.data.content; version = 0} <: member_info bytes)))
   | TNode onp left right -> begin
     tk_left <-- treesync_to_treekem left;
     tk_right <-- treesync_to_treekem right;
@@ -66,67 +49,23 @@ let rec treesync_to_treekem #bytes #cb #l #i t =
       return (TNode (Some kp) tk_left tk_right)
   end
 
-val encrypted_path_secret_tk_to_nt: #bytes:Type0 -> {|crypto_bytes bytes|} -> path_secret_ciphertext bytes -> result (hpke_ciphertext_nt bytes)
-let encrypted_path_secret_tk_to_nt #bytes #cb x =
-  if not (length (x.kem_output <: bytes) < pow2 30) then
-    internal_failure "encrypted_path_secret_tk_to_nt: kem_output too long"
-  else if not (length (x.ciphertext <: bytes) < pow2 30) then
-    internal_failure "encrypted_path_secret_tk_to_nt: ciphertext too long"
-  else
-    return ({
-      kem_output = x.kem_output;
-      ciphertext = x.ciphertext;
-    } <: hpke_ciphertext_nt bytes)
-
-val treekem_to_treesync_node_package: #bytes:Type0 -> {|crypto_bytes bytes|} -> key_package bytes -> result (external_content bytes)
-let treekem_to_treesync_node_package #bytes #cb kp =
-  ciphertexts <-- mapM encrypted_path_secret_tk_to_nt kp.path_secret_ciphertext;
-  if not (bytes_length ps_hpke_ciphertext_nt ciphertexts < pow2 30) then
-    internal_failure "treekem_to_treesync: ciphertexts too long"
-  else if not (length kp.last_group_context < pow2 30) then
-    internal_failure "treekem_to_treesync: last group context too long (internal error)"
-  else begin
-    return ({
-      content = serialize (treekem_content_nt bytes) ({
-        encryption_key = kp.public_key;
-      });
-      impl_data = serialize (treekem_impl_data_nt bytes) ({
-        content_dir = kp.path_secret_from;
-        encrypted_path_secret = ciphertexts;
-        last_group_context = kp.last_group_context;
-      });
-    } <: external_content bytes)
-  end
-
-// Some remarks about the `new_leaf_package` argument
-// This function is used in two cases:
-// - By processing an update path coming from the network. In that case, the update path provided a new leaf package to use, which will go in this `new_leaf_package` argument.
-//   Why change its public key in that case? Well it doesn't really change, because the public key in `PLeaf` and the public key of `new_leaf_package` will be the same.
-//   This is because the `PLeaf` content is equal to `key_package_to_treekem kp` and `new_leaf_package` is equal to `key_package_to_treesync kp` for the same kp
-//   The parent hash extension and the signature will be checked when converting the external_pathsync to a pathsync
-// - When we generate an updatepath, and convert it to treesync before converting it to an update_path_nt.
-//   In that case, `new_leaf_package` need to be equal to our previous leaf package. The HPKE public key will be updated here.
-//   The parent hash and signature need to be updated, but this will be done in the external_pathsync -> pathsync conversion.
-val treekem_to_treesync: #bytes:Type0 -> {|crypto_bytes bytes|} -> #l:nat -> #i:tree_index l -> #li:leaf_index l i -> leaf_package_t bytes -> pathkem bytes l i li -> result (external_pathsync bytes l i li)
+//This function is used to authenticate data generated by TreeKEM. It allows TreeSync to handle parent hash + signature.
+val treekem_to_treesync: #bytes:Type0 -> {|crypto_bytes bytes|} -> #l:nat -> #i:tree_index l -> #li:leaf_index l i -> leaf_node_nt bytes tkt -> pathkem bytes l i li -> result (external_pathsync bytes tkt l i li)
 let rec treekem_to_treesync #bytes #cb #l #i #li new_leaf_package pk =
   match pk with
   | PLeaf mi ->
     return (PLeaf ({
       new_leaf_package with
-      version = (mi <: member_info bytes).version;
-      content = {
-        content = serialize (treekem_content_nt bytes) ({
-          encryption_key = (mi <: member_info bytes).public_key;
-        });
-        impl_data = empty;
+      data = {
+        new_leaf_package.data with
+        content = mi.public_key;
       };
-    } <: leaf_package_t bytes))
+    } <: leaf_node_nt bytes tkt))
   | PNode okp pk_next ->
     next <-- treekem_to_treesync new_leaf_package pk_next;
     match okp with
     | Some kp -> (
-      np <-- treekem_to_treesync_node_package kp;
-      return (PNode (Some np) next)
+      return (PNode (Some kp.public_key) next)
     )
     | None -> (
       return (PNode None next)
