fstar/MLS.TreeCommon.fst
@@ -1,0 +1,86 @@
+module MLS.TreeCommon
+
+open MLS.Tree
+
+#set-options "--fuel 1 --ifuel 1"
+
+(*** Tree creation ***)
+
+val create_tree: #leaf_t:Type -> #node_t:Type -> leaf_t -> tree (option leaf_t) (option node_t) 0 0
+let create_tree lp =
+  TLeaf (Some lp)
+
+(*** Common tree operations ***)
+
+val tree_blank_path: #leaf_t:Type -> #node_t:Type -> #l:nat -> #i:tree_index l -> tree (option leaf_t) (option node_t) l i -> leaf_index l i -> option leaf_t -> tree (option leaf_t) (option node_t) l i
+let rec tree_blank_path #leaf_t #node_t #l #i t li opt_lp =
+  match t with
+  | TLeaf _ -> TLeaf opt_lp
+  | TNode opt_node_content left right -> (
+    if is_left_leaf li
+    then TNode None (tree_blank_path left li opt_lp) right
+    else TNode None left (tree_blank_path right li opt_lp)
+  )
+
+val tree_update: #leaf_t:Type -> #node_t:Type -> #l:nat -> #i:tree_index l -> tree (option leaf_t) (option node_t) l i -> leaf_index l i -> leaf_t -> tree (option leaf_t) (option node_t) l i
+let tree_update #leaf_t #node_t #l #i t li lp =
+  tree_blank_path t li (Some lp)
+
+val tree_remove: #leaf_t:Type -> #node_t:Type -> #l:nat -> #i:tree_index l -> tree (option leaf_t) (option node_t) l i -> leaf_index l i -> tree (option leaf_t) (option node_t) l i
+let tree_remove #leaf_t #node_t #l #i t li =
+  tree_blank_path t li None
+
+(*** Tree extension / truncation ***)
+
+val is_tree_empty: #leaf_t:Type -> #node_t:Type -> #l:nat -> #i:tree_index l -> tree (option leaf_t) (option node_t) l i -> bool
+let rec is_tree_empty #leaf_t #node_t #l #i t =
+  match t with
+  | TNode _ left right ->
+    is_tree_empty left && is_tree_empty right
+  | TLeaf (Some _) -> false
+  | TLeaf None -> true
+
+val canonicalize_tree: #leaf_t:Type -> #node_t:Type -> #l:nat -> tree (option leaf_t) (option node_t) l 0 -> (l_res:nat{l_res <= l} & tree (option leaf_t) (option node_t) l_res 0)
+let canonicalize_tree #leaf_t #node_t #l t0 =
+  match t0 with
+  | TLeaf _ -> (|_, t0|)
+  | TNode _ left right ->
+    if is_tree_empty right then (|_, left|)
+    else (|_, t0|)
+
+// Helper functions to add leaf / extend the tree
+
+val find_empty_leaf: #leaf_t:Type -> #node_t:Type -> #l:nat -> #i:tree_index l -> tree (option leaf_t) (option node_t) l i -> option (leaf_index l i)
+let rec find_empty_leaf #leaf_t #node_t #l #i t =
+  match t with
+  | TLeaf (Some _) -> None
+  | TLeaf None -> Some i
+  | TNode _ left right -> (
+    match find_empty_leaf left, find_empty_leaf right with
+    | Some x, _ -> Some x
+    | None, Some x -> Some x
+    | None, None -> None
+  )
+
+val mk_blank_tree: #leaf_t:Type -> #node_t:Type -> l:nat -> i:tree_index l -> Pure (tree (option leaf_t) (option node_t) l i) (requires True) (ensures fun res -> Some? (find_empty_leaf res))
+let rec mk_blank_tree #leaf_t #node_t l i =
+  if l = 0 then TLeaf None
+  else TNode None (mk_blank_tree (l-1) _) (mk_blank_tree (l-1) _)
+
+val add_one_level: #leaf_t:Type -> #node_t:Type -> #l:nat -> tree (option leaf_t) (option node_t) l 0 -> Pure (tree (option leaf_t) (option node_t) (l+1) 0) (requires True) (fun res -> Some? (find_empty_leaf res))
+let add_one_level #leaf_t #node_t #l t =
+  TNode None t (mk_blank_tree l _)
+
+(*** Add helper ***)
+
+val insert_sorted: #a:eqtype{a `subtype_of` int} -> a -> list a -> list a
+let rec insert_sorted #a x l =
+  match l with
+  | [] -> [x]
+  | h::t ->
+    if x < h then
+      x::l
+    else if x = h then
+      l
+    else
+      h::(insert_sorted x t)
